src/Generated/Aws.dfy
@@ -1,0 +1,9 @@
+module {:extern "Dafny.Aws"} Aws {
+    // No content, this just creates the parent module so that
+    // we can add sub-modules.
+
+    // "Dafny" prefix on the extern because we are also generating
+    // code in the "Aws.*" namespace from our Smithy-to-X code
+    // generation and we need these to be separate
+    // TODO: better name than "Dafny"?
+}
