src/Generated/AwsEncryptionSdk.dfy
@@ -1,0 +1,78 @@
+include "../Util/UTF8.dfy"
+include "../StandardLibrary/StandardLibrary.dfy"
+include "../KMS/AmazonKeyManagementService.dfy"
+include "AwsCryptographicMaterialProviders.dfy"
+
+module {:extern "Dafny.Aws.Esdk"} Aws.Esdk {
+    import Crypto
+    import opened UInt = StandardLibrary.UInt
+    import opened Wrappers
+
+    datatype EncryptInput = EncryptInput(
+        nameonly plaintext: seq<uint8>,
+        nameonly encryptionContext: Crypto.EncryptionContext, // TODO Make an option?
+        nameonly materialsManager: Crypto.ICryptographicMaterialsManager,
+        nameonly algorithmSuiteId: Option<Crypto.AlgorithmSuiteId>
+        // TODO reintroduce optional materialsManager and optional keyring
+    )
+    {
+        predicate Valid() {
+            true 
+        }
+    }
+
+    datatype EncryptOutput = EncryptOutput(
+        nameonly ciphertext: seq<uint8>
+        // TODO Hook up additional Encryption outputs
+        // nameonly encryptionContext: Crypto.EncryptionContext,
+        // nameonly algorithmSuiteId: Crypto.AlgorithmSuiteId
+    )
+    {
+        predicate Valid() {
+            true 
+        }
+    }
+
+    datatype DecryptInput = DecryptInput(
+        nameonly ciphertext: seq<uint8>,
+        nameonly materialsManager: Crypto.ICryptographicMaterialsManager
+        // TODO reintroduce optional and keyring
+    )
+    {
+        predicate Valid() {
+            true 
+        }
+    }
+
+    datatype DecryptOutput = DecryptOutput(
+        nameonly plaintext: seq<uint8>
+        // TODO hook up additional decrypt outputs
+        // nameonly encryptionContext: Crypto.EncryptionContext,
+        // nameonly algorithmSuiteId: Crypto.AlgorithmSuiteId
+    )
+    {
+        predicate Valid() {
+            true 
+        }
+    }
+
+    // datatype AwsEncryptionSdkClientConfig = AwsEncryptionSdkClientConfig(
+    //     nameonly commitmentPolicy: string,
+    //     nameonly maxEncryptedEdks: int,
+    //     nameonly configDefaults: ConfigurationDefaults
+    // )
+    // {
+    //     predicate Valid() {
+    //         true
+    //     }
+    // }
+
+    trait {:termination false} IAwsEncryptionSdkClient {
+        method Encrypt(input: EncryptInput) returns (res: Result<EncryptOutput, string>)
+            requires input.Valid()
+        method Decrypt(input: DecryptInput) returns (res: Result<DecryptOutput, string>)
+            requires input.Valid()
+        // TODO I can't seem to find a way to get this to work
+        // static method {:extern "createClient"} createClient(clientConfig: AwsEncryptionSdkClientConfig) returns (res: IAwsEncryptionSdkClient)
+    }
+}
