test/SDK/Keyring/RawAESKeyring.dfy
@@ -11,6 +11,7 @@ include "../../../src/Crypto/AESEncryption.dfy"
 include "../../../src/StandardLibrary/StandardLibrary.dfy"
 include "../../../src/StandardLibrary/UInt.dfy"
 include "../../../src/Util/UTF8.dfy"
+include "../../../src/Generated/AwsCryptographicMaterialProviders.dfy"
 include "../../Util/TestUtils.dfy"
 
 module TestAESKeyring {
@@ -24,6 +25,7 @@ module TestAESKeyring {
   import EncryptionSuites
   import AlgorithmSuite
   import UTF8
+  import Aws.Crypto
   import opened TestUtils
 
   method {:test} TestOnEncryptOnDecryptGenerateDataKey()
@@ -33,19 +35,47 @@ module TestAESKeyring {
     var encryptionContext := TestUtils.SmallEncryptionContext(TestUtils.SmallEncryptionContextVariation.A);
     ExpectSerializableEncryptionContext(encryptionContext);
 
-    var wrappingAlgorithmID := AlgorithmSuite.AES_256_GCM_IV12_TAG16_HKDF_SHA384_ECDSA_P384;
+    var wrappingAlgorithmID := Crypto.ALG_AES_256_GCM_IV12_TAG16_HKDF_SHA384_ECDSA_P384;
     var signingKey := seq(32, i => 0);
-    var encryptionMaterialsIn := Materials.EncryptionMaterials.WithoutDataKeys(encryptionContext, wrappingAlgorithmID, Some(signingKey));
-    var encryptionMaterialsOut :- expect rawAESKeyring.OnEncrypt(encryptionMaterialsIn);
-    expect |encryptionMaterialsOut.encryptedDataKeys| == 1;
+    var encryptionMaterialsIn := Crypto.EncryptionMaterials(
+      encryptionContext:=encryptionContext,
+      algorithmSuiteId:=wrappingAlgorithmID,
+      plaintextDataKey:=None(),
+      encryptedDataKeys:=[],
+      signingKey:=Some(signingKey)
+    );
+    var encryptionMaterialsOut :- expect rawAESKeyring.OnEncrypt(Crypto.OnEncryptInput(materials:=encryptionMaterialsIn));
 
-    var pdk := encryptionMaterialsOut.plaintextDataKey;
-    var edk := encryptionMaterialsOut.encryptedDataKeys[0];
+    //= compliance/framework/raw-aes-keyring.txt#2.7.1
+    //= type=test
+    //# The keyring MUST append the constructed encrypted data key to the
+    //# encrypted data key list in the encryption materials
+    //# (structures.md#encryption-materials).
+
+    //= compliance/framework/raw-aes-keyring.txt#2.7.1
+    //= type=test
+    //# OnEncrypt MUST output the modified encryption materials
+    //# (structures.md#encryption-materials).
+    expect |encryptionMaterialsOut.materials.encryptedDataKeys| == 1;
+
+    var pdk := encryptionMaterialsOut.materials.plaintextDataKey;
+    var edk := encryptionMaterialsOut.materials.encryptedDataKeys[0];
     var verificationKey := seq(32, i => 0);
 
-    var decryptionMaterialsIn := Materials.DecryptionMaterials.WithoutPlaintextDataKey(encryptionContext, wrappingAlgorithmID, Some(verificationKey));
-    var decryptionMaterialsOut :- expect rawAESKeyring.OnDecrypt(decryptionMaterialsIn, [edk]);
-    expect encryptionMaterialsOut.plaintextDataKey == pdk;
+    var decryptionMaterialsIn := Crypto.DecryptionMaterials(
+      encryptionContext:=encryptionContext,
+      algorithmSuiteId:=wrappingAlgorithmID,
+      plaintextDataKey:=None(),
+      verificationKey:=Some(verificationKey)
+    );
+    var decryptionMaterialsOut :- expect rawAESKeyring.OnDecrypt(Crypto.OnDecryptInput(materials:=decryptionMaterialsIn, encryptedDataKeys:=[edk]));
+
+    //= compliance/framework/raw-aes-keyring.txt#2.7.2
+    //= type=test
+    //# If a decryption succeeds, this keyring MUST add the resulting
+    //# plaintext data key to the decryption materials and return the
+    //# modified materials.
+    expect encryptionMaterialsOut.materials.plaintextDataKey == pdk;
   }
 
   method {:test} TestOnEncryptOnDecryptSuppliedDataKey()
@@ -57,34 +87,111 @@ module TestAESKeyring {
 
     var pdk := seq(32, i => 0);
 
-    var wrappingAlgorithmID := AlgorithmSuite.AES_256_GCM_IV12_TAG16_HKDF_SHA384_ECDSA_P384;
+    var wrappingAlgorithmID := Crypto.ALG_AES_256_GCM_IV12_TAG16_HKDF_SHA384_ECDSA_P384;
     var signingKey := seq(32, i => 0);
+    var encryptionMaterialsIn := Crypto.EncryptionMaterials(
+      encryptionContext:=encryptionContext,
+      algorithmSuiteId:=wrappingAlgorithmID,
+      plaintextDataKey:=Some(pdk),
+      encryptedDataKeys:=[],
+      signingKey:=Some(signingKey)
+    );
+    var encryptionMaterialsOut :- expect rawAESKeyring.OnEncrypt(Crypto.OnEncryptInput(materials:=encryptionMaterialsIn));
+    expect |encryptionMaterialsOut.materials.encryptedDataKeys| == 1;
 
-    var encryptionMaterialsIn := Materials.EncryptionMaterials.WithoutDataKeys(encryptionContext, wrappingAlgorithmID, Some(signingKey))
-                                                              .WithKeys(Some(pdk), []);
-    var encryptionMaterialsOut :- expect rawAESKeyring.OnEncrypt(encryptionMaterialsIn);
-    expect |encryptionMaterialsOut.encryptedDataKeys| == 1;
-
-    var edk := encryptionMaterialsOut.encryptedDataKeys[0];
+    var edk := encryptionMaterialsOut.materials.encryptedDataKeys[0];
     var verificationKey := seq(32, i => 0);
 
-    var decryptionMaterialsIn := Materials.DecryptionMaterials.WithoutPlaintextDataKey(encryptionContext, wrappingAlgorithmID, Some(verificationKey));
-    var decryptionMaterialsOut :- expect rawAESKeyring.OnDecrypt(decryptionMaterialsIn, [edk]);
-    expect decryptionMaterialsOut.plaintextDataKey == Some(pdk);
+    var decryptionMaterialsIn := Crypto.DecryptionMaterials(
+      encryptionContext:=encryptionContext,
+      algorithmSuiteId:=wrappingAlgorithmID,
+      plaintextDataKey:=None(),
+      verificationKey:=Some(verificationKey)
+    );
+    var decryptionMaterialsOut :- expect rawAESKeyring.OnDecrypt(Crypto.OnDecryptInput(materials:=decryptionMaterialsIn, encryptedDataKeys:=[edk]));
+
+    //= compliance/framework/raw-aes-keyring.txt#2.7.1
+    //= type=test
+    //# The keyring MUST encrypt the plaintext data key in the encryption
+    //# materials (structures.md#encryption-materials) using AES-GCM.
+    // We demonstrate this by showing OnEncrypt then OnDecrypt gets us the same pdk back.
+    expect decryptionMaterialsOut.materials.plaintextDataKey == Some(pdk);
   }
 
+    method {:test} TestOnDecryptKeyNameMismatch()
+  {
+    var namespace, name := TestUtils.NamespaceAndName(0);
+    var rawAESKeyring := new RawAESKeyringDef.RawAESKeyring(namespace, name, seq(32, i => 0), EncryptionSuites.AES_GCM_256);
+
+    var mismatchName :- expect UTF8.Encode("mismatched");
+    var mismatchedAESKeyring := new RawAESKeyringDef.RawAESKeyring(namespace, mismatchName, seq(32, i => 0), EncryptionSuites.AES_GCM_256);
+
+    var encryptionContext := TestUtils.SmallEncryptionContext(TestUtils.SmallEncryptionContextVariation.A);
+    ExpectSerializableEncryptionContext(encryptionContext);
+
+    var pdk := seq(32, i => 0);
+
+    var wrappingAlgorithmID := Crypto.ALG_AES_256_GCM_IV12_TAG16_HKDF_SHA384_ECDSA_P384;
+    var signingKey := seq(32, i => 0);
+    var encryptionMaterialsIn := Crypto.EncryptionMaterials(
+      encryptionContext:=encryptionContext,
+      algorithmSuiteId:=wrappingAlgorithmID,
+      plaintextDataKey:=Some(pdk),
+      encryptedDataKeys:=[],
+      signingKey:=Some(signingKey)
+    );
+    var encryptionMaterialsOut :- expect mismatchedAESKeyring.OnEncrypt(Crypto.OnEncryptInput(materials:=encryptionMaterialsIn));
+    expect |encryptionMaterialsOut.materials.encryptedDataKeys| == 1;
+
+    var edk := encryptionMaterialsOut.materials.encryptedDataKeys[0];
+    var verificationKey := seq(32, i => 0);
+
+    var decryptionMaterialsIn := Crypto.DecryptionMaterials(
+      encryptionContext:=encryptionContext,
+      algorithmSuiteId:=wrappingAlgorithmID,
+      plaintextDataKey:=None(),
+      verificationKey:=Some(verificationKey)
+    );
+    var decryptionMaterialsOut :- expect rawAESKeyring.OnDecrypt(Crypto.OnDecryptInput(materials:=decryptionMaterialsIn, encryptedDataKeys:=[edk]));
+    expect decryptionMaterialsOut.materials.plaintextDataKey.None?;
+  }
+
+  // TODO test for multiple EDKS for OnDecrypt
+  // TODO possibly test failure for one?
+  // or is it easier to verify this...
+
+  // TODO test with EDK that shouldn't be decrypted, so with another Keyring e.g.
+
+  //= compliance/framework/raw-aes-keyring.txt#2.7.1
+  //= type=test
+  //# If the encryption materials (structures.md#encryption-materials) do
+  //# not contain a plaintext data key, OnEncrypt MUST generate a random
+  //# plaintext data key and set it on the encryption materials
+  //# (structures.md#encryption-materials).
   method {:test} TestOnDecryptNoEDKs()
   {
     var namespace, name := TestUtils.NamespaceAndName(0);
     var rawAESKeyring := new RawAESKeyringDef.RawAESKeyring(namespace, name, seq(32, i => 0), EncryptionSuites.AES_GCM_256);
-    var wrappingAlgorithmID := AlgorithmSuite.AES_256_GCM_IV12_TAG16_HKDF_SHA384_ECDSA_P384;
+    var wrappingAlgorithmID := Crypto.ALG_AES_256_GCM_IV12_TAG16_HKDF_SHA384_ECDSA_P384;
     var encryptionContext := TestUtils.SmallEncryptionContext(TestUtils.SmallEncryptionContextVariation.A);
     var verificationKey := seq(32, i => 0);
-
-    var decryptionMaterialsIn := Materials.DecryptionMaterials.WithoutPlaintextDataKey(encryptionContext, wrappingAlgorithmID, Some(verificationKey));
-    var decryptionMaterialsOut :- expect rawAESKeyring.OnDecrypt(decryptionMaterialsIn, []);
-    expect decryptionMaterialsOut.plaintextDataKey.None?;
+    var decryptionMaterialsIn := Crypto.DecryptionMaterials(
+      encryptionContext:=encryptionContext,
+      algorithmSuiteId:=wrappingAlgorithmID,
+      plaintextDataKey:=None(),
+      verificationKey:=Some(verificationKey)
+    );
+    var decryptionMaterialsOut :- expect rawAESKeyring.OnDecrypt(Crypto.OnDecryptInput(materials:=decryptionMaterialsIn, encryptedDataKeys:=[]));
+    expect decryptionMaterialsOut.materials.plaintextDataKey.None?;
   }
+
+  //= compliance/framework/raw-aes-keyring.txt#2.7.1
+  //= type=test
+  //# The keyring MUST attempt to serialize the encryption materials'
+  //# (structures.md#encryption-materials) encryption context
+  //# (structures.md#encryption-context-1) in the same format as the
+  //# serialization of message header AAD key value pairs (../data-format/
+  //# message-header.md#key-value-pairs).
 
   method {:test} TestOnEncryptUnserializableEC()
   {
@@ -93,34 +200,58 @@ module TestAESKeyring {
     var unserializableEncryptionContext := generateUnserializableEncryptionContext();
     ExpectNonSerializableEncryptionContext(unserializableEncryptionContext);
 
-    var wrappingAlgorithmID := AlgorithmSuite.AES_256_GCM_IV12_TAG16_HKDF_SHA384_ECDSA_P384;
+    var wrappingAlgorithmID := Crypto.ALG_AES_256_GCM_IV12_TAG16_HKDF_SHA384_ECDSA_P384;
     var signingKey := seq(32, i => 0);
-    var encryptionMaterialsIn := Materials.EncryptionMaterials.WithoutDataKeys(unserializableEncryptionContext, wrappingAlgorithmID, Some(signingKey));
-    var encryptionMaterialsOut := rawAESKeyring.OnEncrypt(encryptionMaterialsIn);
+        var encryptionMaterialsIn := Crypto.EncryptionMaterials(
+      encryptionContext:=unserializableEncryptionContext,
+      algorithmSuiteId:=wrappingAlgorithmID,
+      plaintextDataKey:=None(),
+      encryptedDataKeys:=[],
+      signingKey:=Some(signingKey)
+    );
+    var encryptionMaterialsOut := rawAESKeyring.OnEncrypt(Crypto.OnEncryptInput(materials:=encryptionMaterialsIn));
     expect encryptionMaterialsOut.Failure?;
   }
 
+  //= compliance/framework/raw-aes-keyring.txt#2.7.2
+  //= type=test
+  //# The keyring MUST attempt to serialize the decryption materials'
+  //# (structures.md#decryption-materials) encryption context
+  //# (structures.md#encryption-context-1) in the same format as the
+  //# serialization of the message header AAD key value pairs (../data-
+  //# format/message-header.md#key-value-pairs).
   method {:test} TestOnDecryptUnserializableEC()
   {
     // Set up valid EDK for decryption
     var encryptionContext := TestUtils.SmallEncryptionContext(TestUtils.SmallEncryptionContextVariation.A);
     var namespace, name := TestUtils.NamespaceAndName(0);
     var rawAESKeyring := new RawAESKeyringDef.RawAESKeyring(namespace, name, seq(32, i => 0), EncryptionSuites.AES_GCM_256);
-    var wrappingAlgorithmID := AlgorithmSuite.AES_256_GCM_IV12_TAG16_HKDF_SHA384_ECDSA_P384;
+    var wrappingAlgorithmID := Crypto.ALG_AES_256_GCM_IV12_TAG16_HKDF_SHA384_ECDSA_P384;
     var signingKey := seq(32, i => 0);
-    var encryptionMaterialsIn := Materials.EncryptionMaterials.WithoutDataKeys(encryptionContext, wrappingAlgorithmID, Some(signingKey));
-    var encryptionMaterialsOut :- expect rawAESKeyring.OnEncrypt(encryptionMaterialsIn);
-    expect encryptionMaterialsOut.plaintextDataKey.Some?;
-    expect |encryptionMaterialsOut.encryptedDataKeys| == 1;
-    var edk := encryptionMaterialsOut.encryptedDataKeys[0];
+    var encryptionMaterialsIn := Crypto.EncryptionMaterials(
+      encryptionContext:=encryptionContext,
+      algorithmSuiteId:=wrappingAlgorithmID,
+      plaintextDataKey:=None(),
+      encryptedDataKeys:=[],
+      signingKey:=Some(signingKey)
+    );
+    var encryptionMaterialsOut :- expect rawAESKeyring.OnEncrypt(Crypto.OnEncryptInput(materials:=encryptionMaterialsIn));
+    expect encryptionMaterialsOut.materials.plaintextDataKey.Some?;
+    expect |encryptionMaterialsOut.materials.encryptedDataKeys| == 1;
+    var edk := encryptionMaterialsOut.materials.encryptedDataKeys[0];
 
     // Set up EC that can't be serialized
     var unserializableEncryptionContext := generateUnserializableEncryptionContext();
     ExpectNonSerializableEncryptionContext(unserializableEncryptionContext);
     var verificationKey := seq(32, i => 0);
 
-    var decryptionMaterialsIn := Materials.DecryptionMaterials.WithoutPlaintextDataKey(unserializableEncryptionContext, wrappingAlgorithmID, Some(verificationKey));
-    var decryptionMaterialsOut := rawAESKeyring.OnDecrypt(decryptionMaterialsIn, [edk]);
+    var decryptionMaterialsIn := Crypto.DecryptionMaterials(
+      encryptionContext:=unserializableEncryptionContext,
+      algorithmSuiteId:=wrappingAlgorithmID,
+      plaintextDataKey:=None(),
+      verificationKey:=Some(verificationKey)
+    );
+    var decryptionMaterialsOut := rawAESKeyring.OnDecrypt(Crypto.OnDecryptInput(materials:=decryptionMaterialsIn, encryptedDataKeys:=[edk]));
     expect decryptionMaterialsOut.Failure?;
   }
 
